Simplify/Clean up some existing proofs and reusing stdlib
Summary:
Mostly cleanup.

- As we discussed, ee don't need a decidable equality on Maps, so we don't
  need a decidable equality on their image.
- Some of the things about Strings I proved was hidden inside some OrderedType
  modules, let's use that.

Reviewed By: dkgi

Differential Revision: D20222789

fbshipit-source-id: fc7132d85afc6c1468ba485390ad80bef9be9346

docs/formal/python_semantic/Lib/String.v
@@ -1,144 +1,51 @@
-Require Import Arith Ascii String OrderedTypeEx.
+Require Import String.
+Require Import OrderedType OrderedTypeEx.
 
-(* In this module we define a <<less than>> boolean relation
-   on strings using a lexicographic ordering *)
-Fixpoint ltb (s0 s1: string) : bool :=
-  match (s0, s1) with
-  | (EmptyString, EmptyString) => false
-  | (EmptyString, String _ _) => true
-  | (String _ _, EmptyString) => false
-  | (String u us, String v vs) =>
-      if Nat.eqb (nat_of_ascii u) (nat_of_ascii v)
-      then ltb us vs
-      else Nat.ltb (nat_of_ascii u) (nat_of_ascii v)
+(* Wrapper around String_as_OT *)
+Module String_facts := OrderedTypeFacts(String_as_OT).
+
+Definition lt (s1 s2: string) : Prop := String_as_OT.lt s1 s2.
+
+Definition ltb (s1 s2: string) : bool :=
+  match String_facts.lt_dec s1 s2 with 
+  | left _ => true 
+  | right _ => false
 end.
 
-(* <<nat_of_ascii>> is injective *)
-Definition nat_of_ascii_inverse := String_as_OT.nat_of_ascii_inverse.
-
-Lemma ltb_tail_unique a s1 s2 :
-  ltb (String a s1) (String a s2) = true -> ltb s1 s2 = true.
+Lemma ltb_lt: forall s1 s2, lt s1 s2 <-> ltb s1 s2 = true.
 Proof.
-now simpl; rewrite Nat.eqb_refl.
+unfold lt, ltb.
+intros s1 s2; split; intro h.
+- destruct String_facts.lt_dec as [ hdec | hdec ]; [ reflexivity | ].
+  now elim hdec.
+- destruct String_facts.lt_dec as [ hdec | hdec ]; [ | discriminate ].
+  assumption.
 Qed.
 
-Lemma ltb_irrefl: forall s, ltb s s = false.
+Lemma ltb_nlt: forall s1 s2, (~ lt s1 s2) <-> ltb s1 s2 = false.
 Proof.
-induction s as [ | hd tl hi]; simpl in *; [reflexivity | ].
-now rewrite Nat.eqb_refl.
+intros s1 s2; split; intro h.
+- destruct (ltb_lt s1 s2) as [h1 h2].
+  destruct (ltb s1 s2); [ | reflexivity ].
+  now elim (h (h2 refl_equal)).
+- destruct (ltb_lt s1 s2) as [h1 h2].
+  intro hlt.
+  apply h1 in hlt.
+  rewrite h in hlt.
+  discriminate.
 Qed.
 
-Definition leb s1 s2 := orb (ltb s1 s2) (s1 =? s2)%string.
-
-Remark helper: forall n m, n <> m -> n <= m -> n < m.
-Proof.
-intros n m h hle; revert h; induction hle.
-- intro h; now elim h.
-- auto with arith.
-Qed.
-
-Lemma ltb_antisym: forall s1 s2, ltb s1 s2 = negb (leb s2 s1).  
-Proof.
-unfold leb.
-induction s1 as [ | hd1 tl1 hi]; intros [ | hd2 tl2]; simpl in *;
-    try reflexivity.
-case_eq (Nat.eqb (nat_of_ascii hd1) (nat_of_ascii hd2)); intro h.
-- rewrite Nat.eqb_sym, h.
-  rewrite (hi tl2); f_equal.
-  apply Nat.eqb_eq in h.
-  apply nat_of_ascii_inverse in h.
-  now rewrite h, Ascii.eqb_refl.
-- rewrite Nat.eqb_sym, h.
-  assert (hhd: (hd2 =? hd1)%char = false).
-  + apply Nat.eqb_neq in h.
-    now apply Ascii.eqb_neq; intro; subst; apply h.
-  + rewrite hhd, Bool.orb_false_r, Nat.ltb_antisym; f_equal.
-    apply Nat.eqb_neq in h.
-    case_eq (nat_of_ascii hd2 <=? nat_of_ascii hd1); intro h1.
-    * rewrite Nat.leb_antisym in h1.
-      apply Bool.negb_true_iff in h1.
-      apply Nat.ltb_ge in h1.
-      symmetry.
-      apply Nat.ltb_lt.
-      apply helper; [ | assumption ].
-      intro hx; now apply h; subst.
-    * symmetry.
-      apply Nat.ltb_ge.
-      rewrite Nat.leb_antisym in h1.
-      apply Bool.negb_false_iff in h1.
-      apply Nat.ltb_lt in h1.
-      now auto with arith.
-Qed.
-
-Lemma ltb_trans : forall x y z : string,
-  ltb x y = true -> ltb y z = true -> ltb x z = true.
-Proof.
-induction x as [ | u us hi]; intros [ | v vs] [ | w ws];
-    simpl; try discriminate; intros hxy hyz; [ reflexivity | ].
-case_eq (Nat.eqb (nat_of_ascii u) (nat_of_ascii w)); intro huw.
-- case_eq (Nat.eqb (nat_of_ascii u) (nat_of_ascii v)); intro huv;
-    rewrite huv in hxy.
-  + case_eq (Nat.eqb (nat_of_ascii v) (nat_of_ascii w)); intro hvw;
-    rewrite hvw in hyz.
-    * now apply (hi vs ws).
-    * apply Nat.eqb_eq in huw; rewrite huw in huv.
-      apply Nat.eqb_eq in huv; rewrite huv in hvw.
-      rewrite Nat.eqb_refl in hvw; discriminate hvw.
-  + apply Nat.eqb_eq in huw; rewrite huw in hxy, huv.
-    rewrite Nat.eqb_sym in hyz.
-    rewrite huv in hyz.
-    apply Nat.eqb_neq in huv.
-    apply Nat.ltb_lt in hxy.
-    apply Nat.ltb_lt in hyz.
-    elim (lt_irrefl (nat_of_ascii w)).
-    eapply lt_trans; [ now apply hxy | now apply hyz ].
-- case_eq (Nat.eqb (nat_of_ascii u) (nat_of_ascii v)); intro huv;
-    rewrite huv in hxy.
-  + case_eq (Nat.eqb (nat_of_ascii v) (nat_of_ascii w)); intro hvw;
-    rewrite hvw in hyz.
-    * apply Nat.eqb_eq in huv; rewrite huv in huw.
-      apply Nat.eqb_eq in hvw; rewrite hvw in huw.
-      rewrite Nat.eqb_refl in huw; discriminate huw.
-    * now apply Nat.eqb_eq in huv; rewrite huv.
-  + case_eq (Nat.eqb (nat_of_ascii v) (nat_of_ascii w)); intro hvw;
-      rewrite hvw in hyz.
-    * now apply Nat.eqb_eq in hvw; rewrite hvw in hxy.
-    * apply Nat.ltb_lt.
-      apply Nat.ltb_lt in hxy.
-      apply Nat.ltb_lt in hyz.
-      eapply lt_trans; [ now apply hxy | now apply hyz ].
-Qed.
-
-Lemma lt_not_eq : forall x y : string,
-  ltb x y = true -> (x =? y)%string = false.
-Proof.
-induction x as [ | u us hi]; intros [ | v vs]; simpl in *; try discriminate;
-    intro hlt; [reflexivity | ].
-case_eq (Nat.eqb (nat_of_ascii u) (nat_of_ascii v)); intro huv.
-- apply Nat.eqb_eq in huv.
-  apply nat_of_ascii_inverse in huv; subst.
-  rewrite Ascii.eqb_refl.
-  rewrite Nat.eqb_refl in hlt.
-  now apply hi.
-- apply Nat.eqb_neq in huv. 
-  case_eq (Ascii.eqb u v); intro huv2.
-  + apply Ascii.eqb_eq in huv2; subst.
-    now elim huv.
-  + reflexivity.
-Qed.
+Definition lt_trans := String_as_OT.lt_trans.
 
 Lemma lt_ge: forall x y:string, ltb x y = false -> ltb y x = true \/ x = y.
 Proof.
-induction x as [ | u us hi]; intros [ | v vs] hne; simpl in *.
-- now right.
-- discriminate.
-- now left.
-- rewrite Nat.eqb_sym.
-  case_eq (Nat.eqb (nat_of_ascii u) (nat_of_ascii v)); intro huv;
-    rewrite huv in hne.
-  + apply hi in hne as [ h | h]; [left; assumption|right ].
-    now apply Nat.eqb_eq in huv; apply nat_of_ascii_inverse in huv; subst.
-  + apply Nat.ltb_ge in hne.
-    apply Nat.eqb_neq in huv.
-    now left; apply Nat.ltb_lt; intuition.
+intros x y hltb.
+destruct (String_facts.lt_total x y) as [h | [h | h]].
+- apply ltb_lt in h.
+  now rewrite h in hltb; discriminate.
+- now subst; right.
+- apply ltb_lt in h.
+  now left.
 Qed.
+
+Definition lt_not_eq := String_as_OT.lt_not_eq.
