docs/formal/python_semantic/Map.v
@@ -1,6 +1,6 @@
 Require Import Arith Ascii String List Sorted.
 Import ListNotations.
-Require Import Pyre.Lib.String Pyre.Lib.List.
+Require Import Pyre.Lib.List Pyre.Lib.String.
 
 (** In this module, we define the main <<State>> structure of our judgements.
 The underlying structure is a <<Map>> indexed by <<string>>s. They are
@@ -13,13 +13,8 @@ Section SortedListHelpers.
 Variable A: Type.
 
 (* Pair comparison by only using the first member *)
-Definition pair_ltb (elt0 elt1: string * A) : bool :=
-  ltb (fst elt0) (fst elt1)
-.
-
-(* Propositional equivalent of the boolean relation pair_ltb *)
 Definition pair_lt (elt0 elt1: string * A) : Prop :=
-  pair_ltb elt0 elt1 = true
+  String.lt (fst elt0) (fst elt1)
 .
 
 (* begin hide *)
@@ -32,10 +27,10 @@ now unfold pair_lt in *.
 Qed.
 
 Lemma pair_lt_trans: forall (x y z: string * A),
-  pair_ltb x y = true -> pair_ltb y z = true -> pair_ltb x z = true.
+  pair_lt x y -> pair_lt y z -> pair_lt x z.
 Proof.
-intros [x0 x1] [y0 y1] [z0 z1]; unfold pair_ltb; intros h0 h1; simpl in *.
-now apply ltb_trans with (y := y0).
+intros [x0 x1] [y0 y1] [z0 z1]; intros h0 h1; simpl in *.
+now apply String.lt_trans with (y := y0).
 Qed.
 
 Lemma Forall_pair_lt: forall key1 value1 key2 value2,
@@ -67,83 +62,11 @@ Context {A: Set}.
     encoded as sorted lists of pairs *)
 Record Map : Set := mkMap {
   data :> list (string * A); (* Maps can be coerced to their data field *)
-  correct : Sortedb _ (pair_ltb _) data = true;
+  correct : @Sorted _ (pair_lt _) data
 }.
 
-(* Note to the curious reader: <<Map>> is a dependently typed struct as
-   its <<correct>> field depends on its <<data>> field. So comparing two
-   instances of <<Map>> would require comparing proofs, which is notably
-   hard/impossible to do. However in this particular case, the proof is
-   simply an equality on booleans, which are equipped with a decidable
-   equality. In this case, it is known that we have `uniqueness of identify
-   proofs`, meaning that we won't have to compare anything, as there is a
-   single inhabitant of these types. This allows us to compare maps
-   just as if they were only simply typed lists *)
-
-
-(* A comes with a boolean equality *)
-Variable Aeqb : A -> A -> bool.
-Hypothesis Aeqb_eq: forall x y, Aeqb x y = true -> x = y.
-Hypothesis Aeqb_neq: forall x y, Aeqb x y = false -> x <> y.
-Hypothesis Aeqb_refl: forall x, Aeqb x x = true.
-
-(* Equality over pairs of string * A *)
-Definition pair_eq elt1 elt2 : bool :=
-  (((fst elt1) =? (fst elt2))%string &&
-   Aeqb (snd elt1) (snd elt2))%bool.
-
-(* begin hide *)
-Lemma pair_eq_eq: forall x y, pair_eq x y = true -> x = y.
-Proof.
-intros [k1 v1] [k2 v2] heq.
-apply andb_prop in heq as [h1 h2]; simpl in *.
-apply String.eqb_eq in h1 as ->.
-now apply Aeqb_eq in h2 as ->.
-Qed.
-
-Lemma pair_eq_neq: forall x y, pair_eq x y = false -> x <> y.
-Proof.
-intros [k1 v1] [k2 v2] hneq h; subst.
-injection h; intros; subst; clear h.
-apply Bool.andb_false_iff in hneq; simpl in *.
-destruct hneq as [h | h].
-- now apply String.eqb_neq in h.
-- now apply Aeqb_neq in h.
-Qed.
-
-Lemma pair_eq_refl: forall x, pair_eq x x = true.
-Proof.
-intros [k v]; unfold pair_eq; simpl.
-now rewrite Aeqb_refl, String.eqb_refl.
-Qed.
-(* begin hide *)
-
-(** Boolean equality on <<Map>>s *)
-(* As stated in the previous note, we only compare the underlying list,
-   because of the uniqueness of identity proofs.
-   Note that we also rely on the coercion from map to (data map) provided
-   by the system. The "full" statement should be
-   ``eqb _ pair_eq (data map1) (data map2)`` but this version is a bit 
-   more readable *)
-Definition eqb (map1 map2: Map) : bool :=
-  (eqb _ pair_eq map1 map2).
-
-Lemma eqb_eq: forall map1 map2, eqb map1 map2 = true -> map1 = map2.
-Proof.
-intros [l1 h1] [l2 h2] h; unfold eqb in h; simpl in *.
-apply List.eqb_eq in h as ->; [ | now apply pair_eq_eq].
-now rewrite (sorted_proof_unicity _ _ l2 _ h1 h2).
-Qed.
-
-Lemma eqb_neq: forall map1 map2, eqb map1 map2 = false -> map1 <> map2.
-Proof.
-intros [l1 h1] [l2 h2] hn h; unfold eqb in hn; simpl in *.
-injection h; clear h; intros; subst.
-rewrite List.eqb_refl in hn; [ discriminate | now apply pair_eq_refl].
-Qed.
-
 (** The empty map *)
-Definition empty: Map := mkMap nil (refl_equal _).
+Definition empty: Map := mkMap nil (Sorted_nil _).
 
 (** Reading from a map, might return None if the key is not present *)
 Fixpoint get_map_ (map: list (string * A)) id : option A :=
@@ -168,7 +91,7 @@ Fixpoint insert_sorted (key: string) (value: A)
   | (key', value') :: l' =>
       if (key =? key')%string
       then (key, value) :: l'
-      else if ltb key key'
+      else if String.ltb key key'
            then (key, value) :: l
            else (key', value') :: insert_sorted key value l'
   end.
@@ -177,12 +100,12 @@ Fixpoint insert_sorted (key: string) (value: A)
 Lemma insert_sorted_hdrel: forall l key value,
   HdRel (pair_lt _) (key, value) l ->
   forall key' value',
-  ltb key key' = true ->
+  String.lt key key' ->
   HdRel (pair_lt _) (key, value) (insert_sorted key' value' l).
 Proof.
 induction l as [ | [k v] data hi]; intros key value hhd key' value' hlt;
     simpl in *; [now constructor | ].
-apply HdRel_inv in hhd; unfold pair_lt, pair_ltb in hhd; simpl in hhd.
+apply HdRel_inv in hhd; unfold pair_lt in hhd; simpl in hhd.
 case_eq (String.eqb key' k); intro heq.
 - now constructor.
 - case_eq (ltb key' k); intro hk;  now constructor.
@@ -200,29 +123,22 @@ case_eq (String.eqb key' key); intro heq.
   now apply HdRel_pair_lt_right with (value0 := value).
 - case_eq (ltb key' key); intro hkeys.
   + constructor; [ assumption | ].
+    apply String.ltb_lt in hkeys.
     now constructor; unfold pair_lt; simpl.
   + apply Sorted_inv in hsort as [ h0 h1].
     constructor; [ now apply hi | ].
     apply insert_sorted_hdrel;[ assumption | ].
     apply String.eqb_neq in heq.
-    apply lt_ge in hkeys as [ h | h ]; [assumption | ].
+    apply String.lt_ge in hkeys as [ h | h ]; [ now apply String.ltb_lt | ].
     now elim heq.
 Qed.
-
-Lemma insert_sorted_sorts_bool: forall l, Sortedb _ (pair_ltb _) l = true ->
-  forall key value, Sortedb _ (pair_ltb _) (insert_sorted key value l) = true.
-Proof.
-intros l h key value.
-apply reflect_Sorted in h; apply reflect_Sorted.
-now apply insert_sorted_sorts.
-Qed.
-(* begin hide *)
+(* end hide *)
 
 (** Set a <<key>> to some <<value>> in a <<Map>>, overriding the existing
     value if the <<key>> was already in use. *)
 Definition set_map (map: Map) key (value: A) : Map := 
   let new_data := insert_sorted key value map in
-  mkMap new_data (insert_sorted_sorts_bool map (correct map) key value).
+  mkMap new_data (insert_sorted_sorts map (correct map) key value).
 
 (** Removing a key/value pair in a sorted list, based on the key.
     Since we are stricly sorted, the first one (if any) is the only one *)
@@ -270,27 +186,13 @@ apply Sorted_StronglySorted; [| assumption].
 intros x y z.
 now apply pair_lt_trans.
 Qed.
-
-Lemma remove_sorted_sorts_bool: forall l, Sortedb _ (pair_ltb _) l = true ->
-  forall key, Sortedb _ (pair_ltb _) (remove_sorted l key) = true.
-Proof.
-intros l hs key.
-apply reflect_Sorted in hs; apply reflect_Sorted.
-now apply remove_sorted_sorts.
-Qed.
 (* end hide *)
 
 (** Remove an entry from a map. Once this function terminates, the <<key>>
   is no longer mapped to anything in the map. *)
 Definition unset_map (map: Map) key : Map :=
   let new_data := remove_sorted (data map) key in 
-  mkMap new_data (remove_sorted_sorts_bool (data map) (correct map) key).
-
-(** In this section, we proove that our maps enjoy the extensionality
-    property: it is enough to compare all keys to test the equality 
-    between maps.
-    This part reallies on the fact that our <<lt>> relation is transitive. *)
-Section Extensionality.
+  mkMap new_data (remove_sorted_sorts (data map) (correct map) key).
 
 (* If a <<key>> is less that all the keys in a list, then getting <<key>>
    from the list will return nothing. *)
@@ -300,75 +202,13 @@ Proof.
 induction l as [ | [k v] l hi]; intros key value hf; simpl in *; [reflexivity | ].
 case_eq (String.eqb key k); intro hk.
 - apply Forall_inv in hf.
-  unfold pair_lt, pair_ltb in hf; simpl in hf.
-  apply lt_not_eq in hf; rewrite hf in hk; discriminate.
+  unfold pair_lt in hf; simpl in hf.
+  apply String.lt_not_eq in hf.
+  elim hf.
+  now apply String.eqb_eq.
 - apply Forall_inv_tail in hf.
   now apply hi in hf.
 Qed.
-
-(* If two lists are strongly sorted, and all keys map to the same value (or 
-   absence of value, then they are equal. *)
-Lemma map_extensionality_: forall l1 l2,
-  StronglySorted (pair_lt _) l1 ->
-  StronglySorted (pair_lt _) l2 ->
-  (forall key, get_map_ l1 key = get_map_ l2 key) ->
-  l1 = l2.
-Proof.
-induction l1 as [ | [k1 v1] l1 hi]; intros [ | [k2 v2] l2] hs1 hs2 hk;
-    simpl in *.
-- reflexivity.
-- specialize hk with k2.
-  rewrite String.eqb_refl in hk.
-  discriminate hk.
-- specialize hk with k1.
-  rewrite String.eqb_refl in hk.
-  discriminate hk.
-- apply StronglySorted_inv in hs1 as [hs1 hf1].
-  apply StronglySorted_inv in hs2 as [hs2 hf2].
-  case_eq (String.eqb k1 k2); intro hk12.
-  + replace k2 with k1 in * by now apply String.eqb_eq in hk12.
-    rewrite (hi l2); intuition.
-    * replace v2 with v1; [ reflexivity | ].
-      specialize hk with k1.
-      rewrite String.eqb_refl in hk.
-      now injection hk.
-    * specialize hk with key.
-      case_eq (String.eqb key k1); intro heq; rewrite heq in hk; [| assumption].
-      apply String.eqb_eq in heq; subst.
-      now rewrite (get_lt_none l1 k1 v1), (get_lt_none l2 k1 v2).
-  + case_eq (ltb k1 k2); intro hcomp.
-    * specialize hk with k1.
-      rewrite String.eqb_refl, hk12 in hk.
-      rewrite (get_lt_none l2 k1 v1) in hk; [discriminate | ].
-      eapply Forall_pair_lt; [ | apply hf2].
-      now apply hcomp.
-    * specialize hk with k2.
-      rewrite String.eqb_sym in hk12.
-      rewrite String.eqb_refl, hk12 in hk.
-      rewrite (get_lt_none l1 k2 v2) in hk; [discriminate | ].
-      eapply Forall_pair_lt; [ | apply hf1].
-      unfold pair_lt, pair_ltb; simpl.
-      apply lt_ge in hcomp as [ ? | heq]; [assumption | ].
-      subst; rewrite String.eqb_refl in hk12; discriminate.
-Qed.
- 
-(** If two maps have the exact same mappings, they are equal. *)
-Lemma map_extensionality: forall map1 map2,
-  (forall key, get_map map1 key = get_map map2 key) -> map1 = map2.
-Proof.
-intros map1 map2 hk.
-apply eqb_eq.
-destruct map1 as [l1 hl1]; destruct map2 as [l2 hl2];
-   unfold eqb, get_map in *; simpl in *.
-replace l2 with l1; [ now apply List.eqb_refl; apply pair_eq_refl | ].
-apply map_extensionality_; intuition.
-- apply Sorted_StronglySorted; [now intros x y z; apply pair_lt_trans | ].
-  now apply reflect_Sorted.
-- apply Sorted_StronglySorted; [now intros x y z; apply pair_lt_trans | ].
-  now apply reflect_Sorted.
-Qed.
-
-End Extensionality.
 
 Lemma get_set_map: forall map x y a,
   get_map (set_map map x a) y =
@@ -380,7 +220,7 @@ case_eq (String.eqb x k); intro hk; simpl.
 - case_eq (String.eqb y x); intro hyx; rewrite hyx in *; [reflexivity | ].
   apply String.eqb_eq in hk as ->.
   now rewrite hyx.
-- apply andb_prop in hs as [hs hhd].
+- apply Sorted_inv in hs as [hs hhd].
   case_eq (ltb x k); intro hlt; simpl.
   + now case_eq (String.eqb y x); intro hyx; rewrite hyx in *.
   + case_eq (String.eqb y x); intro hyx; rewrite hyx in *.
@@ -399,14 +239,13 @@ Proof.
 unfold unset_map, get_map; simpl.
 intros [l hs] x z.
 induction l as [ | [k v] l hi]; simpl in *; [ now destruct String.eqb | ].
-apply andb_prop in hs as [hs hhd].
+apply Sorted_inv in hs as [hs hhd].
 case_eq (z =? x)%string; intro hzx; rewrite hzx in hi.
 - case_eq (x =? k)%string; intro hxk; simpl.
   + apply String.eqb_eq in hzx.
     apply String.eqb_eq in hxk; subst.
     apply get_lt_none with (value := v).
-    apply HdRel_Forall; [ now apply pair_lt_trans | now apply reflect_Sorted in hs |].
-    now apply reflect_HdRel in hhd.
+    now apply HdRel_Forall; [ now apply pair_lt_trans | | ].
   + apply String.eqb_eq in hzx; subst.
     rewrite hxk.
     now apply hi.
@@ -415,78 +254,6 @@ case_eq (z =? x)%string; intro hzx; rewrite hzx in hi.
     now rewrite hzx.
   + case_eq (z =? k)%string; intro hzk; simpl; [ reflexivity | ].
     now apply hi.
-Qed.
-
-(* Sorted insertion in a sorted list commutes if both keys are different *)
-Lemma set_set_diff_: forall map x y a b z,
-  (x =? y)%string = false ->
-  get_map_ (insert_sorted y b (insert_sorted x a map)) z =
-  get_map_ (insert_sorted x a (insert_sorted y b map)) z.
-Proof.
-induction map as [ | [key value] tl hi]; intros x y a b z hne; simpl in *.
-- rewrite hne, String.eqb_sym, hne.
-  case_eq (ltb y x); intro hlt.
-  + rewrite ltb_antisym in hlt.
-    unfold leb in hlt.
-    rewrite Bool.negb_orb in hlt.
-    apply andb_prop in hlt as [ h1 h2 ].
-    now apply Bool.negb_true_iff in h1 as ->.
-  + rewrite ltb_antisym in hlt.
-    unfold leb in hlt.
-    rewrite Bool.negb_orb in hlt.
-    apply Bool.andb_false_iff in hlt as [ h | h ].
-    * now apply Bool.negb_false_iff in h as ->.
-    * apply Bool.negb_false_iff in h. 
-      rewrite h in hne; discriminate.
-- case_eq (String.eqb x key); intro hxkey; simpl.
-  + apply String.eqb_eq in hxkey; subst.
-    rewrite String.eqb_sym, hne; simpl.
-    case_eq (ltb y key); intro hlt; simpl insert_sorted.
-    * rewrite hne, ltb_antisym; unfold leb.
-      now rewrite hlt, String.eqb_refl.
-    * now rewrite String.eqb_refl.
-  + case_eq (String.eqb y key); intro hykey.
-    * apply String.eqb_eq in hykey; subst.
-      case_eq (ltb x key); intro hlt; simpl insert_sorted.
-      -- rewrite String.eqb_sym, hne, String.eqb_refl, ltb_antisym.
-         now unfold leb; rewrite hlt; simpl.
-      -- now rewrite String.eqb_refl, hne, hlt.
-    * case_eq (ltb x key); intro hltx.
-      -- case_eq (ltb y key); intro hlty; simpl insert_sorted.
-         ++ rewrite String.eqb_sym, hne, hykey, hlty, hxkey, hltx.
-            case_eq (ltb y x); intro h.
-            ** now rewrite ltb_antisym; unfold leb; rewrite h.
-            ** now rewrite ltb_antisym; unfold leb; rewrite h,
-                 String.eqb_sym, hne.
-         ++ rewrite String.eqb_sym, hne, hykey, hlty, hxkey, hltx.
-            case_eq (ltb y x); intro h; [ | reflexivity ].
-            assert (hw: ltb y y = true);
-                  [ | now rewrite ltb_irrefl in hw; discriminate ].
-            apply (ltb_trans y x y); [ assumption | ].
-            apply (ltb_trans x key y); [ assumption | ].
-            now rewrite ltb_antisym; unfold leb; rewrite hlty, hykey.
-     -- case_eq (ltb y key); intro hlty; simpl insert_sorted.
-        ++ rewrite hykey, hne, hlty, hltx, hxkey.
-           case_eq (ltb x y); intro h; [| reflexivity ].
-            assert (hw: ltb x x = true);
-                  [ | now rewrite ltb_irrefl in hw; discriminate ].
-            apply (ltb_trans x y x); [ assumption | ].
-            apply (ltb_trans y key x); [ assumption | ].
-            now rewrite ltb_antisym; unfold leb; rewrite hltx, hxkey.
-        ++ rewrite hykey, hxkey, hlty, hltx.
-           simpl.
-           case_eq (String.eqb z key); [ reflexivity | intro h].
-           now apply hi.
-Qed.
-
-Lemma set_set_diff_map: forall map x y a b,
-  String.eqb x y = false ->
-  set_map (set_map map x a) y b =
-  set_map (set_map map y b) x a.
-Proof.
-intros map x y a b hne; apply map_extensionality; intros z.
-unfold set_map, get_map; simpl.
-now apply set_set_diff_.
 Qed.
 
 (** Intermediate "state", which will be used to track types or values
@@ -523,23 +290,10 @@ intros s x z; unfold unset0, get0; simpl.
 now rewrite get_unset_map.
 Qed.
 
-Lemma set0_set0_diff: forall s x y a b,
-  (x =? y)%string = false ->
-  set0 (set0 s x a) y b =
-  set0 (set0 s y b) x a.
-Proof.
-intros s x y a b hne; unfold set0, get0; simpl.
-now rewrite set_set_diff_map.
-Qed.
-
 End Map.
 
 Section RawState.
 Context {A B: Set}.
-
-Variable Aeqb : A -> A -> bool.
-Hypothesis Aeqb_eq: forall x y, Aeqb x y = true -> x = y.
-Hypothesis Aeqb_refl: forall x, Aeqb x x = true.
 
 (** Main "state", which stores a <<RawState0>> plus additional information
   (like a list of the already checked/defined functions.
@@ -575,17 +329,6 @@ Lemma get_unset:
 Proof.
 intros s x z; unfold unset, get; simpl.
 now rewrite get0_unset0.
-Qed.
-
-Lemma set_set_diff: forall s x y a b,
-  (x =? y)%string = false ->
-  set (set s x a) y b =
-  set (set s y b) x a.
-Proof.
-intros [s ?] x y a b h; simpl.
-unfold set, get.
-simpl state.
-now rewrite (set0_set0_diff _ Aeqb_eq Aeqb_refl).
 Qed.
 
 End RawState.
