docs/formal/python_semantic/Eval.v
@@ -162,8 +162,6 @@ Record func : Set := mkFun {
     name: string;
     (* TODO(T53097965): support more parameter kinds *)
     parameters: list (string * Typ.t);
-    (* All parameters names are distinct from each other *)
-    unique_parameters: NoDup (map fst parameters);
     (* decorators: Expression.t list; *)
     return_annotation: Typ.t; (* no option, set to TNone if need be *)
     (* async: bool; *)
@@ -201,42 +199,17 @@ induction arguments as [ | arg arguments hi];
 now rewrite (hi _ _ _ h).
 Qed.
 
-Lemma prepare_call_state_set: forall now arguments parameters after,
-  prepare_call_state now arguments parameters = Some after ->
-  forall id v,
-  ~ List.In id (List.map fst parameters) ->
-  prepare_call_state (set0 now id v) arguments parameters = Some (set0 after id v).
-Proof.
-intros now arguments; revert now.
-induction arguments as [ | arg argumentss hi]; intros now [ | [name ?] parameters]
-    after h id v hnotin; simpl in *; try discriminate.
-- now injection h; intros; subst.
-- apply hi with (id := id) (v := v) in h.
-  + replace (set0 (set0 now id v) name arg) with
-            (set0 (set0 now name arg) id v); [ assumption | ].
-    apply set0_set0_diff with (Aeqb := Value.eqb); [ now apply Value.eqb_eq |
-        now apply Value.eqb_refl | ].
-    case_eq (String.eqb name id); intro heq; [ | reflexivity ].
-    apply String.eqb_eq in heq.
-    rewrite heq in hnotin.
-    now elim hnotin; left.
-  + intro hin; apply hnotin; now right.
-Qed.
-
 Lemma prepare_call_state_same_length: forall now arguments parameters,
   List.length arguments = List.length parameters ->
-  NoDup (map fst parameters) ->
   exists after, prepare_call_state now arguments parameters = Some after.
 Proof.
 intros now arguments; revert now.
 induction arguments as [ | arg arguments hi]; intros now [ | [name ?] params]
-    hlen hnodup; simpl in *; try discriminate.
+    hlen; simpl in *; try discriminate.
 - now exists now.
-- injection hlen; clear hlen; intro hlen.
-  inversion hnodup; subst; clear hnodup.
-  apply hi with (now := now) in hlen as [after hafter]; [ | assumption ].
-  exists (set0 after name arg); simpl.
-  now rewrite prepare_call_state_set with (after := after).
+- injection hlen; intros; subst; clear hlen.
+  eapply hi in H as [after h].
+  now exists after; exact h.
 Qed.
 
 Definition mkState state info : State := mkRawState state info.
@@ -405,14 +378,8 @@ Definition Ret x := Statement.Return x.
 
 Definition int_id_parameters := ((("x"%string), Typ.Integer) :: nil).
 
-Remark int_id_no_dup: NoDup (map fst int_id_parameters).
-Proof.
-now constructor; [| now constructor].
-Qed.
-
 Definition int_id : func := mkFun "int_id"%string 
   int_id_parameters
-  int_id_no_dup
   Typ.Integer
   (Ret X).
 
@@ -454,7 +421,6 @@ Qed.
 (* Function "expect_int" : int -> void *)
 Definition expect_int : func := mkFun "expect_int"%string 
   int_id_parameters (* we use the same list of parameters *)
-  int_id_no_dup
   Typ.None
   Statement.Pass.
 
